{
 "cells": [
  {
   "cell_type": "markdown",
   "id": "f59791e1",
   "metadata": {},
   "source": [
    "# Problem 1\n",
    "\n",
    "a. By the Master Theorem, $T(n) = \\Theta(n^4)$.\n",
    "\n",
    "b. By the Master Theorem, $T(n) = \\Theta(n)$.\n",
    "\n",
    "c. By the Master Theorem, $T(n) = \\Theta(n^2 \\lg n)$.\n",
    "\n",
    "d. By the Master Theorem, $T(n) = \\Theta(n^2)$.\n",
    "\n",
    "e. By the Master Theorem, $T(n) = \\Theta(n^{\\lg7})$.\n",
    "\n",
    "f. By the Master Theorem, $T(n) = \\Theta(\\sqrt{n} \\lg n)$.\n",
    "\n",
    "g. It is easy to see that the answer should be $\\Theta(n^3)$ by comparing the recursion with the recursion $T(n) = T(n-1) + \\Theta (n^2 )$.\n",
    "\n",
    "# Problem 3\n",
    "\n",
    "a. $S(m) =  2 S ( m/2 ) + \\Theta ( m )$.\n",
    "\n",
    "b. By the Master Method, the solution is $S(m) = \\Theta (m \\lg m ) $.\n",
    "\n",
    "c. The solution is $T(n) = S(\\lg n) = \\Theta (\\lg n \\lg \\lg n )$.\n",
    "\n",
    "e. Consider the substituition $m = \\lg n$. The recursion for the auxilliary function $S$ is $S(m) = 2 S ( m/2 ) + \\Theta ( 1 )$. By the Master Method, the solution is $S(m) = \\Theta ( \\lg m ) $. The solution is $T(n) = S(\\lg n) = \\Theta ( \\lg \\lg n )$.\n",
    "\n",
    "f. Let $m = \\log_3 n$. The recursion for the auxilliary function $S$ is $S(m) = 3 S ( m/3 ) + \\Theta ( 3^m )$. By the Master Method, the solution is $S(m) = \\Theta ( 3^m ) $. The solution is $T(n) = S(\\log_3 n) = \\Theta ( n )$.\n",
    "\n",
    "# Problem 4\n",
    "\n",
    "a. By master theorem, $\\Theta (n^{\\log_3 4})$.\n",
    "\n",
    "b. Let $S(n) = T(n)/n$. Hence $S(n) = 3/n T(n/3) + 1 / \\lg n = S(n/3) + 1 / \\lg n$. We have $S(n) = \\Theta ( \\sum_{i=1}^{n} \\lg i ) = \\Theta ( \\lg \\lg n ). Hence $T(n) = \\Theta (n \\lg \\lg n )$.\n",
    "\n",
    "c. By master theorem, $\\Theta (n^{2.5})$.\n",
    "\n",
    "d. The solution is $\\Theta(n\\text{lg}n)$. The subtraction occurring inside the argument to $T$ won't change the asymptotics of the solution. Once we drop that subtraction, the master theorem yields the solution.\n",
    "\n",
    "e. Same as b.\n",
    "\n",
    "f. \n",
    "\n",
    "g. The integral test implies the answer is $\\Theta ( \\lg n )$.\n",
    "\n",
    "h. Note that $T(n) = \\lg n + \\lg (n-1) + \\cdots + \\lg 1 = \\lg n! = \\Theta (n \\lg n )$.\n",
    "\n",
    "i. The approach is previous parts imply the answer is $\\Theta ( n/\\lg n)$. \n",
    "\n",
    "j. Note that $n^{1/2^k} = 2$ if and only if $k = \\lg \\lg n$.\n",
    "Easy manipulations that the recursion is asymptotically of the form $T(n) = n^{1 - 1/\\lg n} T (2 ) + n \\lg \\lg n$. \n",
    "The solution is $\\Theta ( n \\lg \\lg n ) $.\n",
    "\n",
    "# Problem 5\n",
    "\n",
    "a. \n",
    "\n",
    "$$\n",
    "F(z) \n",
    "= \\sum\\limits_{i=0}^{\\infty} F_i z^i\n",
    "= F_0 + F_1 z + \\sum\\limits_{i=2}^{\\infty} (F_{i-1}+F_{i-2})z^i \n",
    "= z + z\\sum\\limits_{i=2}^{\\infty} F_{i-1}z^{i-1} + z^2\\sum\\limits_{i=2}^{\\infty} F_{i-2}z^{i-2} \n",
    "= z + z\\sum\\limits_{i=1}^{\\infty} F_i z^i + z^2 \\sum\\limits_{i=0}^{\\infty} F_i z^i \n",
    "= z + zF(z) + z^2 F(z)\n",
    "$$\n",
    "\n",
    "b. We have\n",
    "\n",
    "$$\n",
    "F(z)\n",
    "=\n",
    "\\frac{z}{1-z-z^2}\n",
    "$$\n",
    "\n",
    "Factoring the denominator with the quadratic formula shows $1 − z − z^2 = (1 − \\varphi z)(1 − \\widehat{\\varphi}z )$, and the final equality comes from a partial fraction decomposition.\n",
    "\n",
    "c.\n",
    "\n",
    "$$F(z) = \\frac{1}{\\sqrt{5}} \\left(\\frac{1}{1-\\phi z} - \\frac{1}{1-\\hat{\\phi}z}\\right) = \\frac{1}{\\sqrt{5}} \\sum\\limits_{i=0}^{\\infty}(\\phi z)^i - \\frac{1}{\\sqrt{5}} \\sum\\limits_{i=0}^{\\infty}(\\hat{\\phi}z)^i = \\sum\\limits_{i=0}^{\\infty}\\frac{1}{\\sqrt{5}}(\\phi^i - \\hat{\\phi}^i)z^i$$\n",
    "\n",
    "d.\n",
    "\n",
    "From the definition of the generating function, $F_i$ is the coefficient of $z^i$ in $F(z)$. By part (c) this is given by $\\frac{1}{\\sqrt{5}}(\\phi^i - \\hat{\\phi}^i)$. Since $|\\hat{\\phi}| < 1$ we must have $\\left|\\frac{\\hat{\\phi}^i}{\\sqrt{5}}\\right| < \\left|\\frac{\\hat{\\phi}}{\\sqrt{5}}\\right| < \\frac{1}{2}$. Finally, since the Fibonacci numbers are integers we see that the exact solution must be the approximated solution $\\frac{\\phi^i}{\\sqrt{5}}$ rounded to the nearest integer.\n",
    "\n",
    "# Problem 6\n",
    "\n",
    "a. \n",
    "\n",
    "If an array $A$ is Monge then trivially it must satisfy the inequality by taking\n",
    "$k = i + 1$ and $l = j + 1$. Now suppose $A[i, j] + A[i + 1, j + 1] \\leq A[i, j + 1] +\n",
    "A[i + 1, j]$. We'll use induction on rows and columns to show that the array $A$ satisfies the Monge property.\n",
    "Now fix $i$ and $j$, let $r \\geq 1$, and suppose that $A[i, j]+A[i+1, j+r] \\leq A[i, j+r]+A[i+1, j]$.\n",
    "By applying the induction hypothesis and the given inequality, we have:\n",
    "\n",
    "$$\n",
    "A[i, j] + A[i + 1, j + r + 1] \\leq A[i, j + r] + A[i + 1, j] - A[i + 1, j + r] + A[i, j + r + 1] + A[i + 1, j + r] - A[i, j + r] = A[i + 1, j] + A[i, j + r + 1]\n",
    "$$\n",
    "\n",
    "so it follows that we can extend columns and preserve the Monge property.\n",
    "Next we induct on rows. \n",
    "Suppose that $A[i, j] + A[k, l] ≤ A[i, l] + A[k, j]$.\n",
    "Then we have\n",
    "\n",
    "\\begin{align*}\n",
    "A[i, j] + A[k + 1, l] & \\leq A[i, l] + A[k, j] - A[k, l] + A[k + 1, l]  \\\\\n",
    "& \\leq A[i, l] + A[k, j] - A[k, l] + A[k, l] + A[k + 1, l - 1] - A[k, l - 1] \\\\\n",
    "& = A[i, l] + (A[k, j] + A[k + 1, l - 1]) - A[k, l - 1] \\\\\n",
    "& \\leq A[i, l] + A[k, l - 1] + A[k + 1, j] - A[k, l - 1] \\\\\n",
    "& = A[i, l] + A[k + 1, j].\n",
    "\\end{align*}\n",
    "\n",
    "b. Change the 7 to a 5.\n",
    "\n",
    "c. Suppose that there exist $i$ and $k$ such that $i < k$ but $f(i) > f(k)$.  Since $A$ is Monge we must have\n",
    "$A[i, f(k)] + A[k, f(i)] \\leq A[k, f(k)] + A[i, f(i)]$.\n",
    "\n",
    "Since $f(i)$ gives the position of the leftmost minimum element in row $i$, this implies that $A[i, f(i)] < A[i, f(k)]$. \n",
    "Moreover, $A[k, f(k)] \\leq A[k, f(i)]$. \n",
    "Combining these we get $A[k, f(k)] + A[i,f(i)] \\leq A[k,f(i)] + A[i,f(k)]$.\n",
    "This contradicts the Monge array property.\n",
    "\n",
    "d. Based on the conclusion of part c we can restrict the elements which we need to examine. For each odd row $k$ we need only consult the elements between $f(k-1)$ and $f(k+1)$, where we take $f(0) = 1$ and $f(m) = f(m+1) = n$.\n",
    "The matrix has $\\lceil m/2 \\rceil$ odd-numbered rows, and so finding the leftmost minimum of each of them takes:\n",
    "\n",
    "\\begin{equation*}\n",
    "\\sum_{k=1}^{\\lceil m/2 \\rceil} (f(k+1) - f(k-1) + 1) \n",
    "= \\lceil m/2 \\rceil + \\sum_{k=1}^{\\lceil m/2 \\rceil} (f(k+1) - f(k-1))\n",
    "= O(m) + f(m)/f(m+1)\n",
    "= O(m+n)\n",
    "\\end{equation*}\n",
    "\n",
    "e. \n",
    "\n",
    "$$\n",
    "T(m,n) \n",
    "= T(m/2,n) + O(m+n) \n",
    "= T(m/2,n) + am + bn\n",
    "= \\sum_{i=0}^{\\lg m - 1} \\bigg ( \\frac{am}{2^i} + bn \\bigg )\n",
    "\\leq am \\sum_{i=0}^{\\infty} \\frac{1}{2^i} + bn \\lg m\n",
    "=\n",
    "O(m + n \\lg m )\n",
    "$$"
   ]
  },
  {
   "cell_type": "code",
   "execution_count": null,
   "id": "acd3688c",
   "metadata": {},
   "outputs": [],
   "source": []
  },
  {
   "cell_type": "code",
   "execution_count": null,
   "id": "74a5e820",
   "metadata": {},
   "outputs": [],
   "source": []
  }
 ],
 "metadata": {
  "kernelspec": {
   "display_name": "Python 3",
   "language": "python",
   "name": "python3"
  },
  "language_info": {
   "codemirror_mode": {
    "name": "ipython",
    "version": 3
   },
   "file_extension": ".py",
   "mimetype": "text/x-python",
   "name": "python",
   "nbconvert_exporter": "python",
   "pygments_lexer": "ipython3",
   "version": "3.8.8"
  }
 },
 "nbformat": 4,
 "nbformat_minor": 5
}
